Logic/Predicate/Meta.lean
@@ -6,7 +6,7 @@ open Qq Lean Elab Meta Tactic
 namespace SubTerm
 namespace Meta
 
-section lemmas
+section lemmata
 variable {L : Language.{u}} {μ : Type v} {n}
 
 lemma free_fixedVar_last (n : ℕ) : free (#⟨n, Nat.lt.base n⟩ : SyntacticSubTerm L (n + 1)) = &0 :=
@@ -83,6 +83,30 @@ lemma shift_subst {t : SyntacticSubTerm L (n + 1)} {u t' u'}
   simp[←ht, ←hu, shift, SubTerm.subst, map, bind_bind]; congr; funext x
   cases' x using Fin.lastCases with x <;> simp
 
+lemma bShift_func0 (f : L.func 0) :
+    bShift (SubTerm.func (L := L) (μ:= μ) (n := n) f ![]) = SubTerm.func f ![] := by simp
+
+lemma bShift_func1 (f : L.func 1) {t : SubTerm L μ n} {t'} (h : bShift t = t'):
+    bShift (SubTerm.func f ![t]) = SubTerm.func f ![t'] := by simp[←h]; funext x; simp
+
+lemma bShift_func2 (f : L.func 2) {t₁ t₂ : SubTerm L μ n} {t₁' t₂'}
+  (h₁ : bShift t₁ = t₁') (h₂ : bShift t₂ = t₂') :
+    bShift (SubTerm.func f ![t₁, t₂]) = SubTerm.func f ![t₁', t₂'] :=
+  by simp[←h₁, ←h₂]; funext x; cases x using Fin.cases <;> simp
+
+lemma bShift_func3 (f : L.func 3) {t₁ t₂ t₃ : SyntacticSubTerm L n} {t₁' t₂' t₃'}
+  (h₁ : bShift t₁ = t₁') (h₂ : bShift t₂ = t₂') (h₃ : bShift t₃ = t₃') :
+    bShift (SubTerm.func f ![t₁, t₂, t₃]) = SubTerm.func f ![t₁', t₂', t₃'] := by
+  simp[←h₁, ←h₂, ←h₃]; funext x;
+  cases' x using Fin.cases with x <;> simp;
+  cases' x using Fin.cases with x <;> simp
+
+lemma bShift_subst {t : SyntacticSubTerm L (n + 1)} {u t' u'}
+  (ht : bShift t = t') (hu : bShift u = u') :
+    bShift (subst u t) = subst u' t' := by
+  simp[←ht, ←hu, bShift, SubTerm.subst, map, bind_bind]; congr; funext x
+  cases' x using Fin.lastCases with x <;> simp[Fin.succ_castSucc]
+
 lemma func1_congr (f : L.func 1) {t t' : SyntacticSubTerm L n} (h : t = t'):
     SubTerm.func f ![t] = SubTerm.func f ![t'] := by simp[←h]
 
@@ -105,26 +129,32 @@ lemma subst_congr_eq {s s' : SubTerm L μ n} {t t' u} (es : s = s') (et : t = t'
 lemma shift_congr_eq {t t' : SyntacticSubTerm L n} {u} (e : t = t') (h : shift t' = u) :
   shift t = u := Eq.trans (congr_arg _ e) h
 
+lemma bShift_congr_eq {t t' : SubTerm L μ n} {u} (e : t = t') (h : bShift t' = u) :
+  bShift t = u := Eq.trans (congr_arg _ e) h
+
 section
 variable [hz : L.HasZero] [ho : L.HasOne] [ha : L.HasAdd]
 
 @[simp] lemma free_natLit (z : ℕ) :
-    free (natLit z : SyntacticSubTerm L (n + 1)) = (natLit z : SyntacticSubTerm L n) :=
+    free (natLit z : SyntacticSubTerm L (n + 1)) = natLit z :=
   SubTerm.bind_natLit _ _ _
 
 @[simp] lemma subst_natLit {s} (z : ℕ) :
-    subst s (natLit z : SubTerm L μ (n + 1)) = (natLit z : SubTerm L μ n) :=
+    subst s (natLit z : SubTerm L μ (n + 1)) = natLit z :=
   SubTerm.bind_natLit _ _ _
 
 @[simp] lemma shift_natLit (z : ℕ) :
-    shift (natLit z : SyntacticSubTerm L n) = (natLit z : SyntacticSubTerm L n) :=
+    shift (natLit z : SyntacticSubTerm L n) = natLit z :=
+  SubTerm.bind_natLit _ _ _
+
+@[simp] lemma bShift_natLit (z : ℕ) :
+    bShift (natLit z : SubTerm L μ n) = natLit z :=
   SubTerm.bind_natLit _ _ _
 
 end
-end lemmas
-open SubTerm
+end lemmata
 
-partial def resultFreeSubTerm {L : Q(Language.{u})} {n : Q(ℕ)} : (t : Q(SyntacticSubTerm $L ($n + 1))) →
+partial def resultFree {L : Q(Language.{u})} {n : Q(ℕ)} : (t : Q(SyntacticSubTerm $L ($n + 1))) →
     MetaM ((res : Q(SyntacticSubTerm $L $n)) × Q(SubTerm.free $t = $res))
   | ~q(#$x)                              => do
     let n ←whnf n 
@@ -144,21 +174,23 @@ partial def resultFreeSubTerm {L : Q(Language.{u})} {n : Q(ℕ)} : (t : Q(Syntac
     return ⟨q(&$z), e⟩
   | ~q(SubTerm.func $f ![])              => pure ⟨q(SubTerm.func $f ![]), q(free_func0 $f)⟩
   | ~q(SubTerm.func $f ![$t])            => do
-    let ⟨tn, e⟩ ← resultFreeSubTerm (L := L) (n := n) t
+    let ⟨tn, e⟩ ← resultFree (L := L) (n := n) t
     return ⟨q(SubTerm.func $f ![$tn]), q(free_func1 $f $e)⟩
   | ~q(SubTerm.func $f ![$t₁, $t₂])      => do
-    let ⟨tn₁, e₁⟩ ← resultFreeSubTerm (L := L) (n := n) t₁
-    let ⟨tn₂, e₂⟩ ← resultFreeSubTerm (L := L) (n := n) t₂
+    let ⟨tn₁, e₁⟩ ← resultFree (L := L) (n := n) t₁
+    let ⟨tn₂, e₂⟩ ← resultFree (L := L) (n := n) t₂
     return ⟨q(SubTerm.func $f ![$tn₁, $tn₂]), q(free_func2 $f $e₁ $e₂)⟩
   | ~q(SubTerm.func $f ![$t₁, $t₂, $t₃]) => do
-    let ⟨tn₁, e₁⟩ ← resultFreeSubTerm (L := L) (n := n) t₁
-    let ⟨tn₂, e₂⟩ ← resultFreeSubTerm (L := L) (n := n) t₂
-    let ⟨tn₃, e₃⟩ ← resultFreeSubTerm (L := L) (n := n) t₃
+    let ⟨tn₁, e₁⟩ ← resultFree (L := L) (n := n) t₁
+    let ⟨tn₂, e₂⟩ ← resultFree (L := L) (n := n) t₂
+    let ⟨tn₃, e₃⟩ ← resultFree (L := L) (n := n) t₃
     return ⟨q(SubTerm.func $f ![$tn₁, $tn₂, $tn₃]), q(free_func3 $f $e₁ $e₂ $e₃)⟩
   | ~q(natLit (hz := $hz) (ho := $ho) (ha := $ha) $z) => pure ⟨q(natLit $z), q(free_natLit $z)⟩
-  | ~q($t)                               => pure ⟨q(SubTerm.free $t), q(rfl)⟩
+  | ~q($t)                               => do
+    logInfo m!"match fail: {t}"
+    return ⟨q(SubTerm.free $t), q(rfl)⟩
 
-partial def resultSubstSubTerm {L : Q(Language.{u})} {n : Q(ℕ)} (s : Q(SyntacticSubTerm $L $n)) :
+partial def resultSubst {L : Q(Language.{u})} {n : Q(ℕ)} (s : Q(SyntacticSubTerm $L $n)) :
    (t : Q(SyntacticSubTerm $L ($n + 1))) →
     MetaM ((res : Q(SyntacticSubTerm $L $n)) × Q(SubTerm.subst $s $t = $res))
   | ~q(#$x)                              => do
@@ -175,21 +207,23 @@ partial def resultSubstSubTerm {L : Q(Language.{u})} {n : Q(ℕ)} (s : Q(Syntact
   | ~q(&$x)                              => pure ⟨q(&$x), q(SubTerm.subst_freeVar _ _)⟩
   | ~q(SubTerm.func $f ![])              => pure ⟨q(SubTerm.func $f ![]), q(subst_func0 $f)⟩
   | ~q(SubTerm.func $f ![$t])            => do
-    let ⟨tn, e⟩ ← resultSubstSubTerm (L := L) (n := n) s t
+    let ⟨tn, e⟩ ← resultSubst (L := L) (n := n) s t
     return ⟨q(SubTerm.func $f ![$tn]), q(subst_func1 $f $e)⟩
   | ~q(SubTerm.func $f ![$t₁, $t₂])      => do
-    let ⟨tn₁, e₁⟩ ← resultSubstSubTerm (L := L) (n := n) s t₁
-    let ⟨tn₂, e₂⟩ ← resultSubstSubTerm (L := L) (n := n) s t₂
+    let ⟨tn₁, e₁⟩ ← resultSubst (L := L) (n := n) s t₁
+    let ⟨tn₂, e₂⟩ ← resultSubst (L := L) (n := n) s t₂
     return ⟨q(SubTerm.func $f ![$tn₁, $tn₂]), q(subst_func2 $f $e₁ $e₂)⟩
   | ~q(SubTerm.func $f ![$t₁, $t₂, $t₃]) => do
-    let ⟨tn₁, e₁⟩ ← resultSubstSubTerm (L := L) (n := n) s t₁
-    let ⟨tn₂, e₂⟩ ← resultSubstSubTerm (L := L) (n := n) s t₂
-    let ⟨tn₃, e₃⟩ ← resultSubstSubTerm (L := L) (n := n) s t₃
+    let ⟨tn₁, e₁⟩ ← resultSubst (L := L) (n := n) s t₁
+    let ⟨tn₂, e₂⟩ ← resultSubst (L := L) (n := n) s t₂
+    let ⟨tn₃, e₃⟩ ← resultSubst (L := L) (n := n) s t₃
     return ⟨q(SubTerm.func $f ![$tn₁, $tn₂, $tn₃]), q(subst_func3 $f $e₁ $e₂ $e₃)⟩
   | ~q(natLit (hz := $hz) (ho := $ho) (ha := $ha) $z) => pure ⟨q(natLit $z), q(subst_natLit $z)⟩
-  | ~q($t)                               => pure ⟨q(SubTerm.subst $s $t), q(rfl)⟩
+  | ~q($t)                               => do
+    logInfo m!"match fail: {t}"
+    return ⟨q(SubTerm.subst $s $t), q(rfl)⟩
 
-partial def resultShiftSubTerm {L : Q(Language.{u})} {n : Q(ℕ)} : (t : Q(SyntacticSubTerm $L $n)) →
+partial def resultShift {L : Q(Language.{u})} {n : Q(ℕ)} : (t : Q(SyntacticSubTerm $L $n)) →
     MetaM ((res : Q(SyntacticSubTerm $L $n)) × Q(SubTerm.shift $t = $res))
   | ~q(#$x)                              => pure ⟨q(#$x), q(SubTerm.shift_fixedVar $x)⟩
   | ~q(&$x)                              =>  do
@@ -198,62 +232,93 @@ partial def resultShiftSubTerm {L : Q(Language.{u})} {n : Q(ℕ)} : (t : Q(Synta
     return ⟨q(&$z), e⟩
   | ~q(SubTerm.func $f ![])              => pure ⟨q(SubTerm.func $f ![]), q(shift_func0 $f)⟩
   | ~q(SubTerm.func $f ![$t])            => do
-    let ⟨tn, e⟩ ← resultShiftSubTerm (L := L) (n := n) t
+    let ⟨tn, e⟩ ← resultShift (L := L) (n := n) t
     return ⟨q(SubTerm.func $f ![$tn]), q(shift_func1 $f $e)⟩
   | ~q(SubTerm.func $f ![$t₁, $t₂])      => do
-    let ⟨tn₁, e₁⟩ ← resultShiftSubTerm (L := L) (n := n) t₁
-    let ⟨tn₂, e₂⟩ ← resultShiftSubTerm (L := L) (n := n) t₂
+    let ⟨tn₁, e₁⟩ ← resultShift (L := L) (n := n) t₁
+    let ⟨tn₂, e₂⟩ ← resultShift (L := L) (n := n) t₂
     return ⟨q(SubTerm.func $f ![$tn₁, $tn₂]), q(shift_func2 $f $e₁ $e₂)⟩
   | ~q(SubTerm.func $f ![$t₁, $t₂, $t₃]) => do
-    let ⟨tn₁, e₁⟩ ← resultShiftSubTerm (L := L) (n := n) t₁
-    let ⟨tn₂, e₂⟩ ← resultShiftSubTerm (L := L) (n := n) t₂
-    let ⟨tn₃, e₃⟩ ← resultShiftSubTerm (L := L) (n := n) t₃
+    let ⟨tn₁, e₁⟩ ← resultShift (L := L) (n := n) t₁
+    let ⟨tn₂, e₂⟩ ← resultShift (L := L) (n := n) t₂
+    let ⟨tn₃, e₃⟩ ← resultShift (L := L) (n := n) t₃
     return ⟨q(SubTerm.func $f ![$tn₁, $tn₂, $tn₃]), q(shift_func3 $f $e₁ $e₂ $e₃)⟩
   | ~q(SubTerm.subst $t₁ $t₂)            => do
-    let ⟨tn₁, e₁⟩ ← resultShiftSubTerm (L := L) (n := n) t₁
-    let ⟨tn₂, e₂⟩ ← resultShiftSubTerm (L := L) (n := q(.succ $n)) t₂
+    let ⟨tn₁, e₁⟩ ← resultShift (L := L) (n := n) t₁
+    let ⟨tn₂, e₂⟩ ← resultShift (L := L) (n := q(.succ $n)) t₂
     return ⟨q(SubTerm.subst $tn₁ $tn₂), q(shift_subst $e₂ $e₁)⟩
   | ~q(natLit (hz := $hz) (ho := $ho) (ha := $ha) $z) => pure ⟨q(natLit $z), q(shift_natLit $z)⟩
   | ~q($t)                               => do
-    pure ⟨q(shift $t), q(rfl)⟩
+    logInfo m!"match fail: {t}"
+    return ⟨q(shift $t), q(rfl)⟩
 
-partial def resultSubTerm {L : Q(Language.{u})} {n : Q(ℕ)} : (t : Q(SyntacticSubTerm $L $n)) →
+partial def resultBShift {L : Q(Language.{u})} {n : Q(ℕ)} : (t : Q(SyntacticSubTerm $L $n)) →
+    MetaM ((res : Q(SyntacticSubTerm $L ($n + 1))) × Q(bShift $t = $res))
+  | ~q(#$x)                              => do
+    let z ← natAppFunQ Nat.succ x
+    let e := q(SubTerm.fixedSucc_fixedVar (L := $L) (μ := ℕ) (n := $n) $x)
+    return ⟨q(&$z), e⟩
+  | ~q(&$x)                              => pure ⟨q(&$x), q(SubTerm.fixedSucc_freeVar $x)⟩
+  | ~q(SubTerm.func $f ![])              => pure ⟨q(SubTerm.func $f ![]), q(bShift_func0 $f)⟩
+  | ~q(SubTerm.func $f ![$t])            => do
+    let ⟨tn, e⟩ ← resultBShift (L := L) (n := n) t
+    return ⟨q(SubTerm.func $f ![$tn]), q(bShift_func1 $f $e)⟩
+  | ~q(SubTerm.func $f ![$t₁, $t₂])      => do
+    let ⟨tn₁, e₁⟩ ← resultBShift (L := L) (n := n) t₁
+    let ⟨tn₂, e₂⟩ ← resultBShift (L := L) (n := n) t₂
+    return ⟨q(SubTerm.func $f ![$tn₁, $tn₂]), q(bShift_func2 $f $e₁ $e₂)⟩
+  | ~q(SubTerm.func $f ![$t₁, $t₂, $t₃]) => do
+    let ⟨tn₁, e₁⟩ ← resultBShift (L := L) (n := n) t₁
+    let ⟨tn₂, e₂⟩ ← resultBShift (L := L) (n := n) t₂
+    let ⟨tn₃, e₃⟩ ← resultBShift (L := L) (n := n) t₃
+    return ⟨q(SubTerm.func $f ![$tn₁, $tn₂, $tn₃]), q(bShift_func3 $f $e₁ $e₂ $e₃)⟩
+  | ~q(SubTerm.subst $t₁ $t₂)            => do
+    let ⟨tn₁, e₁⟩ ← resultBShift (L := L) (n := n) t₁
+    let ⟨tn₂, e₂⟩ ← resultBShift (L := L) (n := q(.succ $n)) t₂
+    return ⟨q(SubTerm.subst $tn₁ $tn₂), q(bShift_subst $e₂ $e₁)⟩
+  | ~q(natLit (hz := $hz) (ho := $ho) (ha := $ha) $z) => pure ⟨q(natLit $z), q(bShift_natLit $z)⟩
+  | ~q($t)                               => do
+    logInfo m!"match fail: {t}"
+    return ⟨q(bShift $t), q(rfl)⟩
+
+partial def result {L : Q(Language.{u})} {n : Q(ℕ)} : (t : Q(SyntacticSubTerm $L $n)) →
     MetaM ((res : Q(SyntacticSubTerm $L $n)) × Q($t = $res))
   | ~q(#$x)                              => pure ⟨q(#$x), q(rfl)⟩
   | ~q(&$x)                              => pure ⟨q(&$x), q(rfl)⟩
   | ~q(SubTerm.func $f ![])              => pure ⟨q(SubTerm.func $f ![]), q(rfl)⟩
   | ~q(SubTerm.func $f ![$t])            => do
-    let ⟨tn, e⟩ ← resultSubTerm (L := L) (n := n) t
+    let ⟨tn, e⟩ ← result (L := L) (n := n) t
     return ⟨q(SubTerm.func $f ![$tn]), q(func1_congr $f $e)⟩
   | ~q(SubTerm.func $f ![$t₁, $t₂])      => do
-    let ⟨tn₁, e₁⟩ ← resultSubTerm (L := L) (n := n) t₁
-    let ⟨tn₂, e₂⟩ ← resultSubTerm (L := L) (n := n) t₂
+    let ⟨tn₁, e₁⟩ ← result (L := L) (n := n) t₁
+    let ⟨tn₂, e₂⟩ ← result (L := L) (n := n) t₂
     return ⟨q(SubTerm.func $f ![$tn₁, $tn₂]), q(func2_congr $f $e₁ $e₂)⟩
   | ~q(SubTerm.func $f ![$t₁, $t₂, $t₃]) => do
-    let ⟨tn₁, e₁⟩ ← resultSubTerm (L := L) (n := n) t₁
-    let ⟨tn₂, e₂⟩ ← resultSubTerm (L := L) (n := n) t₂
-    let ⟨tn₃, e₃⟩ ← resultSubTerm (L := L) (n := n) t₃
+    let ⟨tn₁, e₁⟩ ← result (L := L) (n := n) t₁
+    let ⟨tn₂, e₂⟩ ← result (L := L) (n := n) t₂
+    let ⟨tn₃, e₃⟩ ← result (L := L) (n := n) t₃
     return ⟨q(SubTerm.func $f ![$tn₁, $tn₂, $tn₃]), q(func3_congr $f $e₁ $e₂ $e₃)⟩
   | ~q(free $t)                          => do
-    let ⟨tn, e⟩ ← resultSubTerm (L := L) (n := q(.succ $n)) t
-    let ⟨tnn, ee⟩ ← resultFreeSubTerm (L := L) (n := n) tn
+    let ⟨tn, e⟩ ← result (L := L) (n := q(.succ $n)) t
+    let ⟨tnn, ee⟩ ← resultFree (L := L) (n := n) tn
     return ⟨q($tnn), q(free_congr_eq $e $ee)⟩
   | ~q(subst $s $t)                      => do
-    let ⟨tn, te⟩ ← resultSubTerm (L := L) (n := q(.succ $n)) t
-    let ⟨sn, se⟩ ← resultSubTerm (L := L) (n := q($n)) s
-    let ⟨tnn, ee⟩ ← resultSubstSubTerm (L := L) (n := n) sn tn
+    let ⟨tn, te⟩ ← result (L := L) (n := q(.succ $n)) t
+    let ⟨sn, se⟩ ← result (L := L) (n := q($n)) s
+    let ⟨tnn, ee⟩ ← resultSubst (L := L) (n := n) sn tn
     return ⟨q($tnn), q(subst_congr_eq $se $te $ee)⟩
   | ~q(shift $t)                         => do
-    let ⟨tn, e⟩ ← resultSubTerm (L := L) (n := q($n)) t
-    let ⟨tnn, ee⟩ ← resultShiftSubTerm (L := L) (n := n) tn
+    let ⟨tn, e⟩ ← result (L := L) (n := q($n)) t
+    let ⟨tnn, ee⟩ ← resultShift (L := L) (n := n) tn
     return ⟨q($tnn), q(shift_congr_eq $e $ee)⟩
   | ~q(natLit (hz := $hz) (ho := $ho) (ha := $ha) $z) => pure ⟨q(natLit $z), q(rfl)⟩
   | ~q($t)                               => do
-    pure ⟨q($t), q(rfl)⟩
+    logInfo m!"match fail: {t}"
+    return ⟨q($t), q(rfl)⟩
 
-partial def resultSubTerm' {L : Q(Language.{u})} {n : Q(ℕ)} (t : Q(SyntacticSubTerm $L $n)) :
+partial def result' {L : Q(Language.{u})} {n : Q(ℕ)} (t : Q(SyntacticSubTerm $L $n)) :
     MetaM (Result (u := u) q(SyntacticSubTerm $L $n) t) := do
-    let ⟨res, e⟩ ← resultSubTerm t 
+    let ⟨res, e⟩ ← result t 
     return ⟨res, e⟩
 
 private inductive ResultTest (α : Type u) : (a : α) → Type u
@@ -266,14 +331,14 @@ elab "dbg" : tactic => do
   logInfo m!"t = {t} : SyntacticSubTerm {L} {n}"
   let t : Q(SyntacticSubTerm $L $n) ← withReducible <| whnf t
 
-  let ⟨tn, e⟩ ← resultSubTerm (L := L) (n := n) t
+  let ⟨tn, e⟩ ← result (L := L) (n := n) t
   logInfo m!"tn = {tn}"
   logInfo m!"e = {e}"
   let c : Q(ResultTest (SyntacticSubTerm $L $n) $t) := (q(ResultTest.result ($t) $tn $e) : Expr)
   Lean.Elab.Tactic.closeMainGoal c
 
 example {t : SyntacticSubTerm Language.oring 13} : ResultTest (SyntacticSubTerm Language.oring 12)
-    (shift $ subst &99 T“(!t) + (#6 * !(free T“#2 + 9”)) + &7”) :=
+    (shift $ subst &99 T“(!t) + (#6 * !(bShift T“#2 + 9”)) + &7”) :=
   by dbg
 
 example : 1 ≠ 2 := of_decide_eq_true rfl
